name component callback provider

rocq/theories/TypeSystem/End2EndSafety.v
@@ -1550,6 +1550,17 @@ Definition strict_exact_closure_component_body_route_package_at_provider
     store_safe_synthetic_direct_call_ready_exact_body_call_route_package_at
       (global_env_with_local_bounds env' (fn_bounds f_component)) fname.
 
+Definition strict_exact_closure_component_body_store_safe_callback_at_provider
+    (env' : global_env) (f_component : fn_def) : Prop :=
+  forall fname args synthetic_body fdef,
+    direct_call_target_expr (fn_body f_component) =
+      Some (fname, args, synthetic_body) ->
+    lookup_fn fname
+      (env_fns (global_env_with_local_bounds env' (fn_bounds f_component))) =
+      Some fdef ->
+    eval_preserves_typing_roots_store_safe_synthetic_direct_call_ready_body_call_store_safe_callback_height_statement_at
+      (global_env_with_local_bounds env' (fn_bounds f_component)) fdef.
+
 Lemma infer_program_env_end2end_strict_exact_closure_component_body_exact_body_route_package_at_of_component_check :
   forall env env' f_component fname args synthetic_body fdef,
     infer_program_env_end2end_strict_exact_closure env = infer_ok env' ->
@@ -3050,14 +3061,8 @@ Theorem infer_program_env_end2end_strict_exact_closure_big_step_safe_checked_ini
       In f_component (env_fns env') ->
       check_fn_root_shadow_no_capture_direct_call_component_store_safe_summary
         env' f_component = true ->
-      (forall fname args synthetic_body fdef,
-        direct_call_target_expr (fn_body f_component) =
-          Some (fname, args, synthetic_body) ->
-        lookup_fn fname
-          (env_fns (global_env_with_local_bounds env' (fn_bounds f_component))) =
-          Some fdef ->
-        eval_preserves_typing_roots_store_safe_synthetic_direct_call_ready_body_call_store_safe_callback_height_statement_at
-          (global_env_with_local_bounds env' (fn_bounds f_component)) fdef) /\
+      strict_exact_closure_component_body_store_safe_callback_at_provider
+        env' f_component /\
       ((forall fname args synthetic_body,
         direct_call_target_expr (fn_body f_component) =
           Some (fname, args, synthetic_body) ->
